programs/lean/Project/FloatRound/Spec.lean
@@ -1,5 +1,4 @@
 import Project.FloatRound.Program
-import CodeLib.IEEE32.Exec
 
 /-!
 # Specification for `float_round`
